src-coc/alg/notations.v
@@ -1,0 +1,148 @@
+Require Export alg.ln_inf.
+Require Export Coq.Unicode.Utf8.
+
+Notation "e1 ⟶′ e2" := (areduce e1 e2) (at level 65) : type_scope.
+
+Declare Scope acontext_scope.
+Delimit Scope acontext_scope with actx.
+Bind Scope acontext_scope with acontext.
+
+Notation "G ,′′ x : A" :=
+  (actx_cons G x A)
+    (at level 58, x at level 0, left associativity) : acontext_scope.
+
+Open Scope acontext_scope.
+
+Declare Scope work_scope.
+Delimit Scope work_scope with work.
+Bind Scope work_scope with work.
+
+Notation "G ⊢′ e1 ~~ e2 ⇐′ A" :=
+  (w_check G e1 e2 A)
+    ( at level 55, e1 at level 50, e2 at level 50
+    , no associativity) : work_scope.
+
+Notation "G ⊢′ e ⇐′ A" :=
+  (w_check G e e A)
+    ( at level 55, e at level 50, no associativity) : work_scope.
+
+Notation "e1 ~~ e2 ⇐′ A" :=
+  (w_check actx_nil e1 e2 A)
+    (at level 55, e2 at level 50, no associativity) : work_scope.
+
+Notation "e ⇐′ A" :=
+  (w_check actx_nil e e A)
+    (at level 55, no associativity) : work_scope.
+
+Notation "e1 ~~ e2 ⇒′ c" :=
+  (w_infer e1 e2 c)
+    (at level 55, e2 at level 50, no associativity) : work_scope.
+
+Notation "e ⇒′ c" :=
+  (w_infer e e c)
+    (at level 55, no associativity) : work_scope.
+
+Notation "A ⋅ e1 & e2 ⇒′ c" :=
+  (w_infer_app A e1 e2 c)
+    ( at level 55, e1 at level 50
+    , e2 at level 50, no associativity) : work_scope.
+
+Notation "A ⧼~~⧽′ B" :=
+  (w_compact A B)
+    (at level 55, no associativity) : work_scope.
+
+Notation "c $′ e" :=
+  (w_apply c e)
+    (at level 55, no associativity) : work_scope.
+
+Declare Scope bind_scope.
+Delimit Scope bind_scope with bind.
+Bind Scope bind_scope with binding.
+
+Notation "x :′ A" :=
+  (b_var x A)
+    (at level 52, no associativity) : bind_scope.
+
+Notation "^ x :′ k" :=
+  (b_ex x k)
+    (x at level 0, at level 52, no associativity) : bind_scope.
+
+Notation "⧼ ^ k ⧽" :=
+  (b_kind k)
+    (k at level 0, at level 0, no associativity) : bind_scope.
+
+Declare Scope worklist_scope.
+Delimit Scope worklist_scope with wl.
+Bind Scope worklist_scope with worklist.
+
+Notation "G ⊨′ w" :=
+  (wl_cons G w) (at level 58, left associativity) : worklist_scope.
+
+Notation "G ,′ b" :=
+  (wl_bind G b) (at level 58, b at level 52, left associativity) : worklist_scope.
+
+Notation "G ,′ ◁" :=
+  (wl_tag G) (at level 58, left associativity) : worklist_scope.
+
+Declare Scope aexpr_scope.
+Delimit Scope aexpr_scope with aexpr.
+Bind Scope aexpr_scope with aexpr.
+
+Notation "`′ x" :=
+  (ae_var_f x) (at level 0, x at level 0, no associativity) : aexpr_scope.
+
+Notation "↑′ n" :=
+  (ae_var_b n) (at level 0, n at level 0) : aexpr_scope.
+
+Notation "e ^`′ x" :=
+  (open_aexpr_wrt_aexpr e (ae_var_f x)) (at level 48, left associativity) : aexpr_scope.
+
+Notation "e1 ^^′ e2" :=
+  (open_aexpr_wrt_aexpr e1 e2) (at level 48, left associativity) : aexpr_scope.
+
+Notation "[ v /^ x ] e" :=
+  (ex_subst_aexpr v x e)
+    (at level 49, v at level 50, x at level 0, right associativity) : aexpr_scope.
+
+Notation "[ v /′ x ] e" :=
+  (subst_aexpr v x e)
+    (at level 49, v at level 50, x at level 0, right associativity) : aexpr_scope.
+
+Notation "[ k /⧼ x ⧽] e" :=
+  (k_subst_aexpr k x e)
+    (at level 49, k at level 50, x at level 0, right associativity) : aexpr_scope.
+
+Notation "⋆′" :=
+  (ae_kind ak_star) (at level 0, no associativity) : aexpr_scope.
+
+Notation "◻′" :=
+  (ae_kind ak_box) (at level 0, no associativity) : aexpr_scope.
+
+Notation "⧼ k ⧽′" :=
+  (ae_kind k) (at level 0, no associativity) : aexpr_scope.
+
+Notation "⧼ `^ x ⧽" :=
+  (ae_kind (ak_ex x)) (at level 0, no associativity) : aexpr_scope.
+
+Notation "`^ x" :=
+  (ae_ex x) (at level 0, x at level 0, no associativity) : aexpr_scope.
+
+Open Scope work_scope.
+Open Scope worklist_scope.
+Open Scope bind_scope.
+Open Scope aexpr_scope.
+
+Declare Scope cont_scope.
+Delimit Scope cont_scope with cont.
+Bind Scope cont_scope with cont.
+
+Notation "'__' ⋅ e1 & e2 ⇒′ c" :=
+  (c_app e1 e2 c)
+    (at level 53, e1 at level 50, e2 at level 50
+      , no associativity) : cont_scope.
+
+Notation "'__' ⧼~~⧽′ A" :=
+  (c_check A)
+    (at level 53, no associativity) : cont_scope.
+
+Open Scope cont_scope.
