src-coc/alg/worklist.v
@@ -1,0 +1,284 @@
+Require Export alg.notations.
+
+Reserved Notation "G1 ⫢′ G2" (at level 58, left associativity).
+Fixpoint wl_app (G1 G2 : worklist) :=
+  match G2 with
+  | wl_nil => G1
+  | G2' ,′ b => G1 ⫢′ G2' ,′ b
+  | G2' ⊨′ b => G1 ⫢′ G2' ⊨′ b
+  | G2' ,′ ◁ => G1 ⫢′ G2' ,′ ◁
+  end
+where "G1 ⫢′ G2" := (wl_app G1 G2) : worklist_scope
+.
+
+Reserved Notation "Γ1 ,,′ Γ2" (at level 58, left associativity).
+Fixpoint actx_app (Γ1 Γ2 : acontext) :=
+  match Γ2 with
+  | actx_nil => Γ1
+  | Γ2' ,′′ x : A => Γ1 ,,′ Γ2' ,′′ x : A
+  end
+where "Γ1 ,,′ Γ2" := (actx_app Γ1 Γ2) : acontext_scope.
+
+Reserved Notation "⌈ Γ ⌉′"
+  (at level 0, Γ at level 58, no associativity).
+Fixpoint to_wl (Γ : acontext) : worklist :=
+  match Γ with
+  | actx_nil => wl_nil
+  | Γ' ,′′ x : A => ⌈ Γ' ⌉′ ,′ x :′ A
+  end
+where "⌈ Γ ⌉′" := (to_wl Γ) : worklist_scope.
+
+Definition binding_var (b : binding) : var :=
+  match b with
+  | x :′ A => x
+  | ^x :′ k => x
+  | ⧼^k⧽ => k
+  end.
+
+Fixpoint wl_dom (Γ : worklist) : atoms :=
+  match Γ with
+  | wl_nil => empty
+  | Γ' ⊨′ w => wl_dom Γ'
+  | Γ' ,′ b => add (binding_var b) (wl_dom Γ')
+  | Γ' ,′ ◁ => wl_dom Γ'
+  end
+.
+
+Reserved Notation "⟦ e /′ ^ x ⟧ G"
+  (at level 56, e at level 50, x at level 0, right associativity).
+Fixpoint subst_ex (e : aexpr) (x : var) (Γ : worklist) : worklist :=
+  match Γ with
+  | wl_nil => wl_nil
+  | Γ' ⊨′ w => ⟦ e /′ ^x ⟧ Γ' ⊨′ ex_subst_work e x w
+  | Γ' ,′ ◁ => ⟦ e /′ ^x ⟧ Γ' ,′ ◁
+  | Γ' ,′ y :′ A => ⟦ e /′ ^x ⟧ Γ' ,′ y :′ [e /^ x] A
+  | Γ' ,′ ⧼^k⧽ => ⟦ e /′ ^x ⟧ Γ' ,′ ⧼^k⧽
+  | Γ' ,′ ^y :′ k =>
+    if eqb x y then Γ'
+      else ⟦ e /′ ^x ⟧ Γ' ,′ ^y :′ k
+  end
+where "⟦ e /′ ^ x ⟧ G" := (subst_ex e x G) : worklist_scope
+.
+
+Reserved Notation "⟦ k /′ ⧼ x ⧽ ⟧ G"
+  (at level 56, k at level 50, x at level 0, right associativity).
+Fixpoint subst_k (k : akind) (x : var) (Γ : worklist) : worklist :=
+  match Γ with
+  | wl_nil => wl_nil
+  | Γ' ⊨′ w => ⟦ k /′ ⧼ x ⧽ ⟧ Γ' ⊨′ k_subst_work k x w
+  | Γ' ,′ ◁ => ⟦ k /′ ⧼ x ⧽ ⟧ Γ' ,′ ◁
+  | Γ' ,′  y :′ A => ⟦ k /′ ⧼ x ⧽ ⟧ Γ' ,′  y :′ [k /⧼ x ⧽] A
+  | Γ' ,′ ^y :′ k' => ⟦ k /′ ⧼ x ⧽ ⟧ Γ' ,′ ^y :′ k_subst_akind k x k'
+  | Γ' ,′ ⧼^y⧽ =>
+    if eqb x y then Γ' else ⟦ k /′ ⧼x⧽ ⟧ Γ' ,′ ⧼^y⧽
+  end
+where "⟦ k /′ ⧼ x ⧽ ⟧ G" := (subst_k k x G) : worklist_scope
+.
+
+Inductive apply_cont : cont → aexpr → worklist → Prop :=
+| apc_app : forall c F e1 e2,
+    apply_cont (c_app e1 e2 c) F
+      (wl_nil ⊨′ F ⋅ e1 & e2 ⇒′ c)
+| apc_done : forall e,
+  apply_cont c_done e wl_nil
+| apc_check : forall A B,
+    apply_cont (c_check B) A
+      (wl_nil ⊨′ A ⧼~~⧽′ B)
+.
+
+(* expression tranform with variables *)
+Definition ev_trans := aexpr → var * aexpr → aexpr → Prop.
+
+Inductive reorder :
+  aexpr → ev_trans → atoms → worklist → worklist → aexpr → worklist → Prop :=
+| r_nil : forall e F s, reorder e F s wl_nil wl_nil e wl_nil
+| r_cons : forall e F s Γ ψ e' Γ' w
+  , reorder e F s Γ ψ e' Γ'
+  → reorder e F s (Γ ⊨′ w) ψ e' (Γ' ⊨′ w)
+| r_var : forall e (F : ev_trans) e' s Γ ψ e'' Γ' x A
+  , F e (pair x A) e'
+  → reorder e' F s Γ ψ e'' Γ'
+  → reorder e' F s (Γ,′ x :′ A) ψ e'' (Γ',′ x :′ A)
+| r_tag : forall e F s Γ ψ e' Γ'
+  , reorder e F s Γ ψ e' Γ'
+  → reorder e F s (Γ ,′ ◁) ψ e' (Γ ,′ ◁)
+| r_ex_move : forall e F s Γ ψ e' Γ' x k
+  , x `in` fex_aexpr e
+  → reorder e F s Γ ψ e' Γ'
+  → reorder e F (s `union` fkv_akind k) (Γ,′ ^x :′ k) (ψ,′ ^x :′ k) e' Γ'
+| r_ex_stay : forall e F s Γ ψ e' Γ' x k
+  , x `notin` fex_aexpr e
+  → reorder e F s Γ ψ e' Γ'
+  → reorder e F s (Γ,′ ^x :′ k) ψ e' (Γ',′ ^x :′ k)
+| r_k_move : forall e F s Γ ψ e' Γ' k
+  , k `in` fkv_aexpr e `union` s
+  → reorder e F s Γ ψ e' Γ'
+  → reorder e F s (Γ,′ ⧼^k⧽) (ψ ,′ ⧼^k⧽) e' Γ'
+| r_k_stay : forall e F s Γ ψ e' Γ' k
+  , k `notin` fkv_aexpr e `union` s
+  → reorder e F s Γ ψ e' Γ'
+  → reorder e F s (Γ,′ ⧼^k⧽) ψ e' (Γ',′ ⧼^k⧽)
+.
+
+Inductive wrap_var : ev_trans :=
+| mk_wrap_var : forall e x A,
+    wrap_var e (pair x A) (ae_pi A (close_aexpr_wrt_aexpr x e)).
+
+Inductive scope_trap : ev_trans :=
+| mk_scope_trap : forall e x A
+  , x `notin` fv_aexpr e
+  → scope_trap e (pair x A) e
+.
+
+Definition cont_apply_reorder
+  (e : aexpr) (Γ ψ : worklist) (e' : aexpr) (Γ' : worklist) :=
+  reorder e wrap_var empty Γ ψ e' Γ'.
+
+Definition ex_inst_reorder
+  (e : aexpr) (Γ ψ Γ' : worklist) :=
+  reorder e scope_trap empty Γ ψ e Γ'.
+
+Hint Unfold cont_apply_reorder ex_inst_reorder : core.
+
+Inductive notags : worklist → Prop :=
+| nt_nil : notags wl_nil
+| nt_cons : forall w Γ, notags Γ → notags (Γ ⊨′ w)
+| nt_bind : forall b Γ, notags Γ → notags (Γ,′ b)
+.
+
+Reserved Notation "⪧′ wl" (at level 65, no associativity).
+Inductive wl_step : worklist -> Prop :=
+| st_nil : ⪧′ wl_nil
+(* decl-like inference *)
+| st_var : forall Γ Γ1 Γ2 x A c
+  , Γ = Γ1 ,′ x :′ A ⫢′ Γ2
+  → ⪧′ Γ ⊨′ c $′ A
+  → ⪧′ Γ ⊨′ `′ x ⇒′ c
+| st_num : forall Γ n c
+  , ⪧′ Γ ⊨′ c $′ ae_int
+  → ⪧′ Γ ⊨′ ae_num n ⇒′ c
+| st_int : forall Γ c
+  , ⪧′ Γ ⊨′ c $′ ⋆′
+  → ⪧′ Γ ⊨′ ae_int ⇒′ c
+| st_star_inf : forall Γ c
+  , ⪧′ Γ ⊨′ c $′ ◻′
+  → ⪧′ Γ ⊨′ ⋆′ ⇒′ c
+| st_app : forall Γ f1 f2 a1 a2 c
+  , ⪧′ Γ ,′ ◁ ⊨′ f1 ~~ f2 ⇒′ c_app a1 a2 c
+  -> ⪧′ Γ ⊨′ ae_app f1 a1 ~~ ae_app f2 a2 ⇒′ c
+| st_pi : forall L Γ A1 A2 B1 B2 c
+  , (forall x, x `notin` L → forall k1, k1 `notin` add x L
+    → forall k2, k2 `notin` add k1 (add x L)
+    → ⪧′ Γ ,′ ⧼^k2⧽
+      ⊨′ (actx_nil ,′′ x : A1) ⊢′ B1 ^`′ x ~~ B2 ^`′ x ⇐′ ⧼`^k2⧽
+      ,′ ⧼^k1⧽ ⊨′ A1 ~~ A2 ⇐′ ⧼`^k1⧽
+      ⊨′ c $′ ⧼`^k2⧽)
+  → ⪧′ Γ ⊨′ ae_pi A1 B1 ~~ ae_pi A2 B2 ⇒′ c
+| st_abs : forall L Γ e1 e2 c
+  , (forall x, x `notin` L → forall k, k `notin` add x L
+    → forall A, A `notin` add k (add x L)
+      → ⪧′ Γ ,′ ⧼^k⧽ ,′ ^A :′ ak_ex k ,′ x :′ `^A
+          ⊨′ e1 ^`′ x ~~ e2 ^`′ x ⇒′ c)
+  → ⪧′ Γ ⊨′ ae_abs e1 ~~ ae_abs e2 ⇒′ c
+| st_iapp_pi : forall L Γ A B e1 e2 c
+  , (forall x, x `notin` L → forall k, k `notin` add x L
+    → ⪧′ Γ ⊨′ c $′ B ^^′ e1 ⊨′ e1 ~~ e2 ⇐′ A)
+  → ⪧′ Γ ⊨′ ae_pi A B ⋅ e1 & e2 ⇒′ c
+
+| st_iapp_ex : forall L Γ x k c Γ1 Γ2 e1 e2
+  , Γ = Γ1 ,′ ^x :′ k ⫢′ Γ2
+  → (forall A, A `notin` L → forall B, B `notin` add A L
+    → forall k', k' `notin` add A (add B L)
+      → forall F, F = ae_pi `^A `^B
+        → ⪧′ Γ1 ,′ ⧼^k'⧽ ,′ ^A :′ ak_ex k' ,′ ^B :′ k
+          ⫢′ ex_subst_worklist F x (Γ2 ⊨′ F ⋅ e1 & e2 ⇒′ c))
+  → ⪧′ Γ ⊨′ `^x ⋅ e1 & e2 ⇒′ c
+
+(* ex vars *)
+| st_ex_eq : forall Γ Γ1 x k Γ2 c
+  , Γ = Γ1 ,′ ^x :′ k ⫢′ Γ2
+  → ⪧′ Γ ⊨′ c $′ ae_kind k
+  → ⪧′ Γ ⊨′ `^x ~~ `^x ⇒′ c
+| st_ex_l : forall Γ Γ1 x k Γ2 ψ Γ2' e c
+  , e <> `^ x
+  → Γ = Γ1,′ ^x :′ k ⫢′ Γ2
+  → ex_inst_reorder e Γ2 ψ Γ2'
+  → ⪧′ Γ1 ⫢′ ψ ⊨′ e ⇐′ ⧼ k ⧽′
+      ⫢′ ex_subst_worklist e x (Γ2' ⊨′ c $′ ⧼k⧽′)
+  → ⪧′ Γ ⊨′ `^x ~~ e ⇒′ c
+| st_ex_r : forall Γ Γ1 x k Γ2 ψ Γ2' e c
+  , e <> `^ x
+  → Γ = Γ1,′ ^x :′ k ⫢′ Γ2
+  → ex_inst_reorder e Γ2 ψ Γ2'
+  → ⪧′ Γ1 ⫢′ ψ ⊨′ e ⇐′ ⧼ k ⧽′
+      ⫢′ ex_subst_worklist e x (Γ2' ⊨′ c $′ ⧼k⧽′)
+  → ⪧′ Γ ⊨′ e ~~ `^x ⇒′ c
+
+(* kind ex infer *)
+| st_kv_eq : forall Γ x c
+  , ⪧′ ⟦ak_star /′ ⧼x⧽⟧ (Γ ⊨′ c $′ ◻′)
+  → ⪧′ Γ ⊨′ ⧼`^x⧽ ~~ ⧼`^x⧽ ⇒′ c
+| st_kv_lr : forall Γ x y c
+  , x <> y
+  → ⪧′ ⟦ak_star /′ ⧼y⧽⟧ ⟦ak_star /′ ⧼x⧽⟧ (Γ ⊨′ c $′ ◻′)
+  → ⪧′ Γ ⊨′ ⧼`^x⧽ ~~ ⧼`^y⧽ ⇒′ c
+| st_kv_l : forall Γ x c
+  , ⪧′ ⟦ak_star /′ ⧼x⧽⟧ (Γ ⊨′ c $′ ◻′)
+  → ⪧′ Γ ⊨′ ⧼`^x⧽ ~~ ⋆′ ⇒′ c
+| st_kv_r : forall Γ x c
+  , ⪧′ ⟦ak_star /′ ⧼x⧽⟧ (Γ ⊨′ c $′ ◻′)
+  → ⪧′ Γ ⊨′ ⋆′ ~~ ⧼`^x⧽ ⇒′ c
+
+(* check *)
+| st_check : forall Γ Γ' e1 e2 A
+  , ⪧′ Γ ⫢′ ⌈ Γ' ⌉′,′ ◁ ⊨′ e1 ~~ e2 ⇒′ c_check A
+  → ⪧′ Γ ⊨′ Γ' ⊢′ e1 ~~ e2 ⇐′ A
+
+| st_comp_box_l : forall Γ1 Γ2 k
+  , ⪧′ Γ1 ⫢′ k_subst_worklist ak_box k Γ2
+  → ⪧′ Γ1 ,′ ⧼^k⧽ ⫢′ Γ2 ⊨′ ◻′ ⧼~~⧽′ ⧼`^k⧽
+| st_comp_box_r : forall Γ1 Γ2 k
+  , ⪧′ Γ1 ⫢′ k_subst_worklist ak_box k Γ2
+  → k `notin` wl_dom Γ1 `union` wl_dom Γ2
+  → ⪧′ Γ1 ,′ ⧼^k⧽ ⫢′ Γ2 ⊨′ ⧼`^k⧽ ⧼~~⧽′ ◻′
+| st_comp_kv_eq : forall Γ Γ1 Γ2 k
+  , Γ = Γ1 ,′ ⧼^k⧽ ⫢′ Γ2
+  → ⪧′ Γ
+  → ⪧′ Γ ⊨′ ⧼`^k⧽ ⧼~~⧽′ ⧼`^k⧽
+| st_comp_kv : forall Γ1 Γ2 Γ3 x y
+  , y `notin` add x (wl_dom Γ1 `union` wl_dom Γ2 `union` wl_dom Γ3)
+  → ⪧′ Γ1,′ ⧼^x⧽ ⫢′ Γ2 ⫢′ k_subst_worklist (ak_ex x) y Γ3
+  → ⪧′ Γ1 ,′ ⧼^x⧽ ⫢′ Γ2 ,′ ⧼^y⧽ ⫢′ Γ3 ⊨′ ⧼`^x⧽ ⧼~~⧽′ ⧼`^y⧽
+| st_comp_sub : forall L Γ A B
+  , (forall k, A <> ⧼k⧽′)
+  → (forall k, B <> ⧼k⧽′)
+  → (forall k, k `notin` L → ⪧′ Γ,′ ⧼^k⧽ ⊨′ A ~~ B ⇐′ ⧼`^k⧽)
+  → ⪧′ Γ ⊨′ A ⧼~~⧽′ B
+
+| st_app_cont : forall Γ1 Γ2 ψ Γ2' c e e' Γ'
+  , apply_cont c e' Γ'
+  → notags Γ2
+  → cont_apply_reorder e Γ2 ψ e' Γ2'
+  → ⪧′ Γ1 ⫢′ ψ ⫢′ Γ' ⫢′ Γ2'
+  → ⪧′ Γ1 ,′ ◁ ⫢′ Γ2 ⊨′ c $′ e
+
+(* elim bindings *)
+| st_bind_var : forall L Γ x A
+  , x `notin` wl_dom Γ
+  → (forall k, k `notin` L → ⪧′ Γ ,′ ⧼^k⧽ ⊨′ A ⇐′ ⧼`^k⧽)
+  → ⪧′ Γ ,′ x :′ A
+| st_bind_ex : forall Γ x k
+  , x `notin` wl_dom Γ
+  → ⪧′ Γ
+  → ⪧′ Γ ,′ ^x :′ k
+| st_bind_k : forall Γ k
+  , k `notin` wl_dom Γ
+  → ⪧′ Γ
+  → ⪧′ Γ ,′ ⧼^k⧽
+
+where "⪧′ wl" := (wl_step wl) : type_scope
+.
+
+
+#[export]
+Hint Constructors wl_step : core.
