src-coc/completeness.v
@@ -1,0 +1,28 @@
+Require Import alg.worklist.
+Require Import decl.worklist.
+Require Import transfer.
+
+Require Import Equality.
+
+Theorem completeness : forall Γ,
+    ⪧₂ Γ → forall Γ' Θ, nil ⊢ Γ' ⟿₂ Γ ⊣ Θ → ⪧′ Γ'.
+Proof.
+  induction 1; intros Γ_ Θ Trans.
+  - dependent induction Trans.
+    (* all solveable *)
+    + admit.
+    + admit.
+    + admit.
+  - dependent induction Trans.
+      (* main case infer *)
+    + admit.
+    + admit.
+    + admit.
+  - admit.
+  - admit.
+  - admit.
+  - admit.
+  - admit.
+  - admit.
+  - admit.
+Admitted.
