src-coc/decl/correspondence.v
@@ -1,0 +1,62 @@
+Require Import decl.worklist.
+Require Import Program.Equality.
+
+Theorem soundness__infer : forall Γ e c,
+    ⪧ Γ ⊨ e ⇒' c → exists A, ⌊ Γ ⌋ ⊢ e : A ∧ ⪧ Γ ⊨ c $ A.
+Proof.
+  intros.
+  dependent destruction H.
+  - exists A. now split.
+Qed.
+
+Theorem soundness__check : forall Γ e A,
+    ⪧ Γ ⊨ e ⇐' A → ⌊ Γ ⌋ ⊢ e : A.
+Proof.
+  intros.
+  now dependent destruction H.
+Qed.
+
+Lemma to_ctx_to_wl_id : forall Γ,
+    ⌊ ⌈ Γ ⌉ ⌋ = Γ.
+Proof.
+  intros.
+  induction Γ; simpl.
+  - reflexivity.
+  - now rewrite IHΓ.
+Qed.
+
+Theorem completeness : forall Γ e A,
+    Γ ⊢ e : A → ⪧ ⌈ Γ ⌉ ⊨ e ⇐' A.
+Proof.
+  intros.
+  constructor.
+  now rewrite to_ctx_to_wl_id.
+Qed.
+
+Theorem soundness__infer2 : forall Γ e c,
+    ⪧₂ Γ ⊨ e ⇒' c → exists A, ⌊ Γ ⌋ ⊢ e ⇒ A ∧ ⪧ Γ ⊨ c $ A.
+Proof.
+  intros.
+  dependent destruction H.
+  - admit.
+  - admit.
+Admitted.
+
+Theorem soundness__check2 : forall Γ e A,
+    ⪧ Γ ⊨ e ⇐' A → ⌊ Γ ⌋ ⊢ e ⇐ A.
+Proof.
+Admitted.
+
+Theorem completeness2 : forall Γ e A,
+    Γ ⊢ e : A → ⪧₂ ⌈ Γ ⌉ ⊨ e ⇐' A.
+Proof.
+  intros.
+  induction H.
+  - admit.
+  - admit.
+  - admit.
+  - admit.
+  - admit.
+  - admit.
+  -
+Admitted.
