src-coc/decl/notations.v
@@ -1,0 +1,156 @@
+Require Export Unicode.Utf8.
+
+Require Export decl.ln_inf.
+
+Notation "G ⊢ e : A" :=
+  (tp G e A)
+    (at level 60, e at next level, no associativity) : type_scope.
+
+Notation "⊢ G" :=
+  (wf_context G)
+    (at level 60, no associativity) : type_scope.
+
+Notation "⊢₂ G" :=
+  (wf_context2 G)
+    (at level 60, no associativity) : type_scope.
+
+Notation "G ⊢ e ⇐ A" :=
+  (tp2 G e d_check A)
+    (at level 60, e at next level, no associativity) : type_scope.
+
+Notation "G ⊢ e ⇒ A" :=
+  (tp2 G e d_check A)
+    (at level 60, e at next level, no associativity) : type_scope.
+
+Notation "G ⊢ e ⇔ d A" :=
+  (tp2 G e d A)
+    (at level 60, e at next level, d at level 0, no associativity) : type_scope.
+
+Notation "A ⟶ B" := (reduce A B)
+  (at level 60, no associativity) : type_scope.
+
+Declare Scope context_scope.
+Delimit Scope context_scope with ctx.
+Bind Scope context_scope with context.
+
+Notation "G , x : A" :=
+  (ctx_cons G x A)
+    (at level 58, x at level 0, left associativity) : context_scope.
+
+Reserved Notation "G1 ,, G2"
+  (at level 58, left associativity).
+
+Fixpoint ctx_app (Γ1 Γ2 : context) : context :=
+  match Γ2 with
+  | ctx_nil => Γ1
+  | Γ2', x : A => Γ1 ,, Γ2' , x : A
+  end%ctx
+
+where "G1 ,, G2" := (ctx_app G1 G2) : context_scope.
+
+Notation "⟦ v /_ x ⟧ G" :=
+  (subst_context v x G)
+    ( at level 56, v at level 50, x at level 0
+    , right associativity) : context_scope.
+
+Declare Scope expr_scope.
+Delimit Scope expr_scope with expr.
+Bind Scope expr_scope with expr.
+
+Notation "` x" := (e_var_f x)
+  (at level 0, x at level 0, no associativity) : expr_scope.
+Notation "↑ x" := (e_var_b x)
+  (at level 0, x at level 0, no associativity) : expr_scope.
+
+Notation "[ v /_ x ] e" :=
+  (subst_expr v x e)
+    ( at level 49, v at level 50, x at level 0
+    , right associativity) : expr_scope.
+
+Notation "e ^` x" := (open_expr_wrt_expr e (e_var_f x))
+  (at level 48, left associativity) : expr_scope.
+
+Notation "e1 ^^ e2" := (open_expr_wrt_expr e1 e2)
+  (at level 48, left associativity) : expr_scope.
+
+Notation "⋆" := (e_kind k_star)
+  (at level 0, no associativity) : expr_scope.
+
+Notation "◻" := (e_kind k_box) (at level 0, no associativity) : expr_scope.
+
+Notation "⧼ k ⧽" := (e_kind k)
+  (at level 0, no associativity) : expr_scope.
+
+Notation "[ v / x ] e" :=
+  (subst_expr v x e)
+    ( at level 49, v at level 50, x at level 0
+    , right associativity) : expr_scope.
+
+Open Scope context_scope.
+Open Scope expr_scope.
+
+Declare Scope dwork_scope.
+Delimit Scope dwork_scope with dwork.
+Bind Scope dwork_scope with dwork.
+
+Notation "G ⊢' e ⇐ A" :=
+  (dw_check G e A)
+    (at level 55, e at level 50, no associativity) : dwork_scope.
+
+Notation "e ⇐' A" :=
+  (dw_check ctx_nil e A)
+    (at level 55, no associativity) : dwork_scope.
+
+Notation "e ⇒' c" :=
+  (dw_infer e c)
+    (at level 55, no associativity) : dwork_scope.
+
+Notation "A -- s e ⇒ c" :=
+  (dw_infer_app A s e c)
+    ( at level 55, s at level 0, e at level 50, no associativity) : dwork_scope.
+
+Notation "A ∘ e ⇒ c" :=
+  (dw_infer_app A ds_nd e c)
+    ( at level 55, e at level 50, no associativity) : dwork_scope.
+
+Notation "A ⋅ e ⇒ c" :=
+  (dw_infer_app A ds_d e c)
+    ( at level 55, e at level 50, no associativity) : dwork_scope.
+
+Notation "c $ e" :=
+  (dw_apply c e)
+    (at level 55, no associativity) : dwork_scope.
+
+Notation "A ⧼~~⧽ B" :=
+  (dw_compact A B)
+    (at level 55, no associativity) : dwork_scope.
+
+Declare Scope dworklist_scope.
+Delimit Scope dworklist_scope with dwl.
+Bind Scope dworklist_scope with dworklist.
+
+Notation "G ⊨ w" :=
+  (dwl_cons G w) (at level 58, left associativity) : dworklist_scope.
+
+Notation "G ,' x : A" :=
+  (dwl_bind G x A) (at level 58, x at level 0, left associativity) : dworklist_scope.
+
+Notation "G ,' ◁" :=
+  (dwl_tag G) (at level 58, left associativity) : dworklist_scope.
+
+Open Scope dworklist_scope.
+Open Scope dwork_scope.
+
+Declare Scope dcont_scope.
+Delimit Scope dcont_scope with dcont.
+Bind Scope dwork_scope with dcont.
+
+Notation "'__' ⋅ e ⇒ c" :=
+  (dc_app e c)
+    (at level 53, e at level 50, no associativity) : dcont_scope.
+
+Notation "'__' ⧼~~⧽ A" :=
+  (dc_check A)
+    (at level 53, no associativity) : dcont_scope.
+
+Open Scope dcont_scope.
