src-coc/decl/worklist.v
@@ -1,0 +1,157 @@
+Require Export decl.notations.
+Require Import Program.Equality.
+
+Reserved Notation "G1 ⫢ G2" (at level 58, left associativity).
+Fixpoint dwl_app (G1 G2 : dworklist) :=
+  match G2 with
+  | dwl_nil => G1
+  | G2' ,' x : A => G1 ⫢ G2' ,' x : A
+  | G2' ⊨  b => G1 ⫢ G2' ⊨ b
+  | G2' ,' ◁ => G1 ⫢ G2' ,' ◁
+  end
+where "G1 ⫢ G2" := (dwl_app G1 G2) : dworklist_scope
+.
+
+Fixpoint dwl_dom (Γ : dworklist) : atoms :=
+  match Γ with
+  | dwl_nil => {}
+  | Γ ⊨ w => dwl_dom Γ
+  | Γ ,' x : A => add x (dwl_dom Γ)
+  | Γ ,' ◁ => dwl_dom Γ
+  end
+.
+
+Reserved Notation "⌊ wl ⌋" (at level 0, wl at level 58, no associativity).
+Fixpoint to_ctx (Γ : dworklist) : context :=
+  match Γ with
+  | Γ' ⊨ w => ⌊ Γ' ⌋
+  | Γ' ,' x : A => ⌊ Γ' ⌋ , x : A
+  | Γ' ,' ◁ => ⌊ Γ' ⌋
+  | dwl_nil => ctx_nil
+  end
+where "⌊ wl ⌋" := (to_ctx wl) : context_scope.
+
+Reserved Notation "⌈ ctx ⌉" (at level 0, ctx at level 58, no associativity).
+Fixpoint to_wl (Γ : context) : dworklist :=
+  match Γ with
+  | ctx_nil => dwl_nil
+  | Γ, x : A => ⌈ Γ ⌉ ,' x : A
+  end
+where "⌈ ctx ⌉" := (to_wl ctx) : dworklist_scope
+.
+
+Lemma app_to_bctx_distr : forall Γ1 Γ2,
+    ⌊ Γ1 ⫢ Γ2 ⌋ = ⌊ Γ1 ⌋ ,, ⌊ Γ2 ⌋.
+Proof.
+  induction Γ2; simpl; intros; auto.
+  - now rewrite IHΓ2.
+Qed.
+
+
+Fixpoint wrap_expr_wrt_context (Γ : context) (e : expr) :=
+  match Γ with
+  | ctx_nil => e
+  | Γ' , x : A =>
+      wrap_expr_wrt_context Γ' (e_pi A (close_expr_wrt_expr x e))
+  end
+.
+
+Inductive apply_dcont : dcont → expr → dworklist → Prop :=
+| apdc_done : forall e, apply_dcont dc_done e dwl_nil
+| apdc_app : forall A e c,
+    apply_dcont (dc_app e c) A (dwl_nil ⊨ A ⋅ e ⇒ c)
+| apdc_check : forall A B,
+    apply_dcont (dc_check B) A (dwl_nil ⊨ A ⧼~~⧽ B)
+.
+
+Inductive dnotags : dworklist → Prop :=
+| dnt_nil : dnotags dwl_nil
+| dnt_cons : forall Γ w, dnotags Γ → dnotags (Γ ⊨ w)
+| dnt_var : forall Γ x A, dnotags Γ → dnotags (Γ ,' x : A)
+.
+
+Inductive wrap_expr : expr → dworklist → expr → Prop :=
+| wr_nil : forall e, wrap_expr e dwl_nil e
+| wr_cons : forall Γ w e e', wrap_expr e Γ e' → wrap_expr e (Γ ⊨ w) e'
+| wr_var : forall Γ x A e e'
+  , wrap_expr (e_pi A (close_expr_wrt_expr x e)) Γ e'
+  → wrap_expr e (Γ ,' x : A) e'
+.
+
+Reserved Notation "⪧ wl" (at level 60, no associativity).
+Inductive dwl_step : dworklist → Prop :=
+| dst_nil : ⪧ dwl_nil
+| dst_infer : forall Γ e c A
+  , ⌊ Γ ⌋ ⊢ e : A
+  → ⪧ Γ ⊨ c $ A
+  → ⪧ Γ ⊨ e ⇒' c
+| dst_infer_app : forall Γ A c e B
+  , ⌊ Γ ⌋ ⊢ e : A
+  → ⪧ Γ ⊨ c $ B ^^ e
+  → ⪧ Γ ⊨ e_pi A B ⋅ e ⇒ c
+| dst_comp : forall Γ A k
+  , A <> ◻
+  → ⌊ Γ ⌋ ⊢ A : ⧼ k ⧽
+  → ⪧ Γ ⊨ A ⧼~~⧽ A
+| dst_comp_box : forall Γ
+  , ⪧ Γ
+  → ⪧ Γ ⊨ ◻ ⧼~~⧽ ◻
+| dst_check : forall Γ ψ e A
+  , ⌊ Γ ⌋ ,, ψ ⊢ e : A
+  → ⪧ Γ ⊨ ψ ⊢' e ⇐ A
+| dst_app_cont : forall Γ1 Γ2 c e e' Γ'
+  , dnotags Γ2
+  → wrap_expr e Γ2 e'
+  → apply_dcont c e' Γ'
+  → ⪧ Γ1 ⫢ Γ' ⫢ Γ2
+  → ⪧ Γ1,' ◁ ⫢ Γ2 ⊨ c $ e
+| dst_bind : forall Γ x A k
+  , ⪧ Γ
+  → ⌊ Γ ⌋ ⊢ A : ⧼ k ⧽
+  → x `notin` dwl_dom Γ
+  → ⪧ Γ ,' x : A
+where "⪧ wl" := (dwl_step wl) : type_scope
+.
+
+Reserved Notation "⪧₂ wl" (at level 60, no associativity).
+Inductive dwl_step_c : dworklist → Prop :=
+| dst2_nil : ⪧₂ dwl_nil
+| dst2_infer : forall Γ e c A
+  , (⌊ Γ ⌋ ⊢ e ⇒ A)
+  → ¬ (exists f a, e = e_app f a)
+  → ⪧₂ Γ ⊨ c $ A
+  → ⪧₂ Γ ⊨ e ⇒' c
+| dst2_app : forall Γ f e c F
+  , ⪧₂ Γ ⊨ F ⋅ e ⇒ c
+  → ⌊ Γ ⌋ ⊢ f ⇒ F
+  → ⪧₂ Γ ⊨ e_app f e ⇒' c
+| dst2_infer_app : forall Γ A c e B
+  , (⌊ Γ ⌋ ⊢ e ⇐ A)
+  → ⪧₂ Γ ⊨ c $ B ^^ e
+  → ⪧₂ Γ ⊨ e_pi A B ⋅ e ⇒ c
+| dst2_comp : forall Γ A k
+  , A <> ◻
+  → ⌊ Γ ⌋ ⊢ A : ⧼ k ⧽
+  → ⪧₂ Γ ⊨ A ⧼~~⧽ A
+| dst2_comp_box : forall Γ
+  , ⪧₂ Γ
+  → ⪧₂ Γ ⊨ ◻ ⧼~~⧽ ◻
+| dst2_check : forall Γ ψ e A
+  , ⪧₂ Γ ⫢ ⌈ ψ ⌉ ,' ◁ ⊨ e ⇒' __ ⧼~~⧽ A
+  → ⪧₂ Γ ⊨ ψ ⊢' e ⇐ A
+| dst2_app_cont : forall Γ1 Γ2 c e e' Γ'
+  , dnotags Γ2
+  → wrap_expr e Γ2 e'
+  → apply_dcont c e' Γ'
+  → ⪧₂ Γ1 ⫢ Γ' ⫢ Γ2
+  → ⪧₂ Γ1,' ◁ ⫢ Γ2 ⊨ c $ e
+| dst2_bind : forall Γ x A k
+  , ⪧₂ Γ
+  → ⌊ Γ ⌋ ⊢ A ⇒ ⧼ k ⧽
+  → x `notin` dwl_dom Γ
+  → ⪧₂ Γ ,' x : A
+where "⪧₂ wl" := (dwl_step_c wl) : type_scope
+.
+
+#[export]
+Hint Constructors dwl_step dwl_step_c : core.
