src-coc/soundness.v
@@ -1,0 +1,108 @@
+Require Import alg.worklist.
+Require Import decl.worklist.
+Require Import transfer.
+Require Import ln_utils.
+
+Require Import Program.Equality.
+
+Tactic Notation "dd" ident(H) := dependent destruction H.
+
+Ltac gather_all_atoms :=
+  let xs := gather_atoms_with (fun x : atoms => x) in
+  let x  := gather_atoms_with (fun x : atom => singleton x) in
+  let ae := gather_atoms_with
+              (fun e : aexpr =>
+                 fv_aexpr e `union` fex_aexpr e `union` fkv_aexpr e) in
+  let c  := gather_atoms_with
+              (fun c : cont =>
+                 fv_cont c `union` fex_cont c `union` fkv_cont c) in
+  let L := beautify_fset (xs `union` x `union` ae `union` c) in
+  constr:(L).
+
+Ltac decompose_transfer :=
+  match goal with
+  (* wls *)
+  | H : _ ⊢ _ ⊨′ _ ⟿ _ ⊣ _ |- _ => dd H
+  | H : _ ⊢ _ ,′ _ ⟿ _ ⊣ _ |- _ => dd H
+  (* kinds *)
+  | H : _ ⊢ ak_star ~> _ |- _ => dd H
+  | H : _ ⊢ ak_box  ~> _ |- _ => dd H
+  | H : _ ⊢ ak_ex _ ~> _ |- _ => dd H
+  (* exprs *)
+  | H :  _ ⊢ `^ _ ⇝ _ |- _ => dd H
+  (* works *)
+  | H : _ ⊢ _ ~~ _ ⇒′ _ ⇝′ _ |- _ => dd H
+  | H : _ ⊢ _ ~~ _ ⇐′ _ ⇝′ _ |- _ => dd H
+  | H : _ ⊢ _ $′ _  ⇝′ _ |- _ => dd H
+  (* actx *)
+  | H : _ ⊢ actx_nil ⟿′′ _ |- _ => dd H
+  end
+.
+
+Ltac decompose_transfers :=
+  repeat decompose_transfer.
+
+Ltac cleanup_duplication :=
+  match goal with
+  | H : In (⧼^?x⧽= ?k)  (_; ⧼^?x⧽= ?k)  |- _ => clear H
+  | H : In (⧼^?x⧽= ?k1) (_; ⧼^?x⧽= ?k2) |- _ =>
+      apply wf_il_inst_unique_consₖ in H;
+      eauto with wf_il;
+      subst
+  | H : In (^?x :_ ?k1 = ?A1) (_; ^?x :_ ?k2 = ?A2) |- _ =>
+      let Ek := fresh "Ek" in
+      let Ea := fresh "Ea" in
+      apply wf_il_inst_unique_consₓ in H as (Ek & Ea);
+      eauto with wf_il;
+      subst
+  end
+.
+
+Ltac cleanup_duplications :=
+  repeat cleanup_duplication.
+
+Theorem soundness: forall Γ',
+    ⪧′ Γ' → exists Γ Θ, nil ⊢ Γ' ⟿ Γ ⊣ Θ ∧ ⪧ Γ.
+Proof.
+  induction 1.
+  1-5: admit.
+  - destruct IHwl_step as (Γ0 & Θ & Trans & R).
+    admit.
+  - admit.
+  - repeat inst_cofinites_by' gather_all_atoms.
+    destruct H0 as (Γ0 & Θ & Trans & R).
+    decompose_transfers.
+    cleanup_duplications. simpl in *.
+    exists (Γ0 ⊨ e_abs (close_expr_wrt_expr x e5) ⇒ c0), Θ2.
+    split.
+    + admit.
+    + admit.
+  (* app infer *)
+  - repeat inst_cofinites_by' gather_all_atoms.
+    destruct H0 as (Γ0 & Θ & Trans & R).
+    decompose_transfers.
+  - admit.
+  (* ex insts *)
+  - admit.
+  - destruct IHwl_step as (Γ0 & Θ & Trans & R). admit.
+  - admit.
+  (* kind ex *)
+  - admit.
+  - admit.
+  - admit.
+  - admit.
+  (* check *)
+  - admit.
+  - admit.
+  - admit.
+  - admit.
+  - admit.
+  - admit.
+  (* apply cont *)
+  - destruct IHwl_step as (Γ0 & Θ & Trans & R).
+    admit.
+  (* binds *)
+  - admit.
+  - admit.
+  - admit.
+Admitted.
