src-lite/alg/ln_inf_extra.v
@@ -93,3 +93,85 @@ Lemma open_aexpr_fv_aexpr_notin : forall e x v,
 Proof.
   intros. eauto using open_aexpr_fv_aexpr_notin_rec.
 Qed.
+
+Lemma k_subst_aexpr_open_aexpr_wrt_aexpr_rec : forall e2 e1 x k n
+  , k_subst_aexpr k x (open_aexpr_wrt_aexpr_rec n e2 e1)
+    = open_aexpr_wrt_aexpr_rec n
+        (k_subst_aexpr k x e2) (k_subst_aexpr k x e1).
+Proof.
+  intros e2 e1 x k.
+  induction e1 using aexpr_mut with
+    (P0 := (fun b => forall n, k_subst_abody k x (open_abody_wrt_aexpr_rec n e2 b) = open_abody_wrt_aexpr_rec n (k_subst_aexpr k x e2) (k_subst_abody k x b))); simpl; intros;
+    try (rewrite IHe0, IHe1 || rewrite IHe1_1, IHe1_2 || rewrite IHe1); eauto.
+  - destruct (lt_eq_lt_dec n n0). destruct s.
+    all: simpl; auto.
+Qed.
+
+Lemma k_subst_abody_open_abody_wrt_aexpr_rec : forall b e x k n
+  , k_subst_abody k x (open_abody_wrt_aexpr_rec n e b)
+    = open_abody_wrt_aexpr_rec n
+        (k_subst_aexpr k x e) (k_subst_abody k x b).
+Proof.
+  induction b; simpl; intros.
+  now repeat rewrite k_subst_aexpr_open_aexpr_wrt_aexpr_rec.
+Qed.
+
+Lemma k_subst_aexpr_open_aexpr_wrt_aexpr : forall e2 e1 x k
+  , k_subst_aexpr k x (e1 ^^′ e2)
+    = (k_subst_aexpr k x e1) ^^′ (k_subst_aexpr k x e2).
+Proof.
+  intros.
+  apply k_subst_aexpr_open_aexpr_wrt_aexpr_rec.
+Qed.
+
+Lemma k_subst_abody_open_abody_wrt_aexpr : forall b e x k
+  , k_subst_abody k x (open_abody_wrt_aexpr b e)
+    = open_abody_wrt_aexpr
+        (k_subst_abody k x b) (k_subst_aexpr k x e).
+Proof.
+  intros.
+  apply k_subst_abody_open_abody_wrt_aexpr_rec.
+Qed.
+
+Lemma k_subst_aexpr_fresh_eq : forall e k x
+  , x `notin` fkv_aexpr e
+  → k_subst_aexpr k x e = e.
+Proof.
+  intros e k x.
+  induction e using aexpr_mut with
+    (P0 := fun b => x `notin` fkv_abody b → k_subst_abody k x b = b);
+    simpl; intros; try (rewrite IHe1, IHe2 || rewrite IHe0, IHe || rewrite IHe); auto.
+  - destruct k0; simpl; auto.
+    simpl in H. destruct (kx == x); [> .. | subst; auto].
+    assert (kx <> x) by auto.
+    contradiction.
+Qed.
+
+Lemma k_subst_abody_fresh_eq : forall b k x
+  , x `notin` fkv_abody b
+  → k_subst_abody k x b = b.
+Proof.
+  induction b; simpl; intros.
+  repeat rewrite k_subst_aexpr_fresh_eq; auto.
+Qed.
+
+Lemma aexpr_k_subst_open_comm : forall x k e v
+  , x `notin` fkv_aexpr v
+  → (k_subst_aexpr k x e) ^^′ v = k_subst_aexpr k x (e ^^′ v).
+Proof.
+  intros.
+  rewrite k_subst_aexpr_open_aexpr_wrt_aexpr.
+  rewrite (k_subst_aexpr_fresh_eq v ).
+  all: easy.
+Qed.
+
+Lemma abody_k_subst_open_comm : forall x k b v
+  , x `notin` fkv_aexpr v
+    → open_abody_wrt_aexpr (k_subst_abody k x b) v
+      = k_subst_abody k x (open_abody_wrt_aexpr b v).
+Proof.
+  intros.
+  rewrite k_subst_abody_open_abody_wrt_aexpr.
+  rewrite k_subst_aexpr_fresh_eq.
+  all: easy.
+Qed.
